NuDataStructure.thy
@@ -16,47 +16,32 @@ lemma Intro_Cast_I: "\<^bold>c\<^bold>a\<^bold>s\<^bold>t A \<longmapsto> B \<^b
   unfolding Intro_def Cast_def Premise_def by simp
 lemma Dest_Cast_I: "\<^bold>c\<^bold>a\<^bold>s\<^bold>t A \<longmapsto> B \<^bold>w\<^bold>i\<^bold>t\<^bold>h P \<Longrightarrow> \<^bold>p\<^bold>r\<^bold>e\<^bold>m\<^bold>i\<^bold>s\<^bold>e (P \<longrightarrow> Q) \<Longrightarrow> \<^bold>d\<^bold>e\<^bold>s\<^bold>t \<^bold>c\<^bold>a\<^bold>s\<^bold>t A \<longmapsto> B \<^bold>w\<^bold>i\<^bold>t\<^bold>h Q"
   unfolding Dest_def Cast_def Premise_def by simp
-ML \<open>find_first\<close>
 
 
-lemma "\<^bold>p\<^bold>r\<^bold>e\<^bold>m\<^bold>i\<^bold>s\<^bold>e len < length data \<Longrightarrow>
-  \<^bold>c\<^bold>a\<^bold>s\<^bold>t (a \<R_arr_tail> (len,length data,addr),addr \<R_arr_tail> data) \<tycolon> Ref \<lbrace> \<nat>[size_t] \<cross_product> \<nat>[size_t] \<cross_product> Pointer \<rbrace> \<^emph> Array T
+lemma DynLst_I_\<nu>app:
+  "\<^bold>p\<^bold>r\<^bold>e\<^bold>m\<^bold>i\<^bold>s\<^bold>e len \<le> length data \<and> cap = length data \<Longrightarrow>
+  \<^bold>c\<^bold>a\<^bold>s\<^bold>t (a \<R_arr_tail> (len,cap,addr),addr \<R_arr_tail> data) \<tycolon> Ref \<lbrace> \<nat>[size_t] \<cross_product> \<nat>[size_t] \<cross_product> Pointer \<rbrace> \<^emph> Array T
     \<longmapsto> a \<R_arr_tail> take len data \<tycolon> DynLst T"
-  unfolding DynLst_def by (rule Cast_I) \<nu>reason
+  unfolding DynLst_def Cast_def by (cases a, cases addr) (auto simp add: lrep_exps)
+(* unfolding DynLst_def by (rule Cast_I) \<nu>reason *)
 
-ML \<open>Term.dummy_prop\<close>
-ML \<open>Thm.prop_of Drule.dummy_thm\<close>
-\<nu>cast AA: \<open>a \<R_arr_tail> l \<tycolon> DynLst T\<close>
-  \<longmapsto> \<open>\<exists>* addr buf. (a \<R_arr_tail> (length l,length l + length buf,addr),addr \<R_arr_tail> (l @ buf)) \<tycolon> Ref \<lbrace> \<nat>[size_t] \<cross_product> \<nat>[size_t] \<cross_product> Pointer \<rbrace> \<^emph> Array T\<close>
-  \<bullet> DynLst_def D_\<nu>cast
-
-lemma "(\<And>x. \<exists>y. y = x)" proof
-
-lemma "\<^bold>c\<^bold>a\<^bold>s\<^bold>t a \<R_arr_tail> l \<tycolon> DynLst T
-  \<longmapsto> (\<exists>* addr buf. (a \<R_arr_tail> (length l,length l + length buf,addr),addr \<R_arr_tail> (l @ buf)) \<tycolon> Ref \<lbrace> \<nat>[size_t] \<cross_product> \<nat>[size_t] \<cross_product> Pointer \<rbrace> \<^emph> Array T)"
+lemma [\<nu>overload D]:
+  "\<^bold>c\<^bold>a\<^bold>s\<^bold>t a \<R_arr_tail> l \<tycolon> DynLst T
+  \<longmapsto> (\<exists>* buf addr. (a \<R_arr_tail> (length l,length l + length buf,addr),addr \<R_arr_tail> (l @ buf)) \<tycolon> Ref \<lbrace> \<nat>[size_t] \<cross_product> \<nat>[size_t] \<cross_product> Pointer \<rbrace> \<^emph> Array T)"
   unfolding DynLst_def Cast_def
-  
-  
-  apply (rule Cast_I)
-  ML_val \<open>
-val ctx = Config.put Pattern.unify_trace_failure true @{context}
-fun RSNX tha (i, thb) = let open Thm in
-  (case Seq.chop 2 (biresolution (SOME ctx) false [(false, tha)] i thb) of
-    ([th], _) => solve_constraints th
-  | ([], _) => raise THM ("RSN: no unifiers", i, [tha, thb])
-  | _ => raise THM ("RSN: multiple unifiers", i, [tha, thb]))
-end
+  apply (auto simp add: lrep_exps)
+  subgoal for v len base ofs list
+    by (rule exI[of _ "drop len list"]) (auto simp add: min_absorb1 min_absorb2)
+  done
+
+proc DynLst_new: \<open>R\<heavy_comma> buf_size \<tycolon> \<nat>[size_t]\<heavy_comma> \<^bold>h\<^bold>e\<^bold>a\<^bold>p H\<close> \<longmapsto> \<open>\<exists>*ptr. (R\<heavy_comma> ptr \<tycolon> Pointer\<heavy_comma> \<^bold>h\<^bold>e\<^bold>a\<^bold>p H \<heavy_asterisk> ptr \<R_arr_tail> [] \<tycolon> DynLst T)\<close>
+  requires \<open>\<^bold>p\<^bold>a\<^bold>r\<^bold>a\<^bold>m T\<close>
+        and [\<nu>intro]: \<open>\<nu>Zero T zero\<close>
+  \<bullet> \<rightarrow> buf_size
+  \<bullet> alloc \<open>\<lbrace> \<nat>[size_t] \<cross_product> \<nat>[size_t] \<cross_product> Pointer \<rbrace>\<close>
+  \<bullet> buf_size \<down>: 2 buf_size alloc_array \<open>T\<close> \<down>: 3 DynLst_I
+  finish
 
 
-val x= RSNX @{thm BBB} (1, #goal @{Isar.goal})
-\<close>
-   apply (\<nu>reason) unfolding Premise_def
-  apply auto
-ML \<open>find_first\<close>
-notepad
-begin
-  assume  A[simplified (no_asm_simp)]: "id ((a,b,c) = (a',b',c')) \<Longrightarrow> P (a,b,c)"
-end
-
-
+ML \<open>Runtime.exn_trace\<close>
 end
